BmapAllocAll: prove the multi-blockmap allocator correct
also, change the BmapAllocAll API slightly.

instead of encoding the free block into a single number, the
BmapAllocAll API returns the block as a (blockmapnum,blockmapoff)
pair.  the next level will encode them into a single block number.

src/BmapAllocAllMod.v
@@ -15,29 +15,31 @@ Open Scope fscq.
 Module BmapAllocAll <: SmallStepLang.
 
 Inductive prog {R:Type} : Type :=
-  | Alloc (rx:option BlocksPartDisk.addr->prog)
-  | Free (a:BlocksPartDisk.addr) (rx:unit->prog)
+  | Alloc (rx:option (blockmapnum*blockmapoff)->prog)
+  | Free (a:blockmapnum) (off:blockmapoff) (rx:unit->prog)
   | Return (v:R).
 Definition Prog := @prog.
 Definition ReturnOp := @Return.
-Definition State := BlocksPartDisk.addr -> AllocState.
-
-Definition freebit (bm:State) (off:BlocksPartDisk.addr) :=
-  bm off = Avail.
+Definition State := blockmapnum -> blockmap.
 
 Inductive step {R:Type} : @progstate R Prog State ->
                           @progstate R Prog State -> Prop :=
-  | StepAllocOK: forall d off rx,
-    highest (freebit d) off ->
+  | StepAllocOK: forall d bn off rx,
+    highest (fun bn' => exists off', BmapAllocOne.freebit (d bn') off') bn ->
+    highest (BmapAllocOne.freebit (d bn)) off ->
     step (PS (Alloc rx) d)
-         (PS (rx (Some off)) (setidx BlocksPartDisk.eq_addr_dec d off InUse))
+         (PS (rx (Some (bn, off)))
+             (setidx eq_blockmapnum_dec d bn
+              (setidx eq_blockmapoff_dec (d bn) off InUse)))
   | StepAllocOut: forall d rx,
-    (~exists off, freebit d off) ->
+    (~exists bn off, BmapAllocOne.freebit (d bn) off) ->
     step (PS (Alloc rx) d)
          (PS (rx None) d)
-  | StepFree: forall d off rx,
-    step (PS (Free off rx) d)
-         (PS (rx tt) (setidx BlocksPartDisk.eq_addr_dec d off Avail)).
+  | StepFree: forall d bn off rx,
+    step (PS (Free bn off rx) d)
+         (PS (rx tt)
+             (setidx eq_blockmapnum_dec d bn
+              (setidx eq_blockmapoff_dec (d bn) off Avail))).
 Definition Step := @step.
 
 End BmapAllocAll.
@@ -47,7 +49,111 @@ Module BmapAllocAllToAllocOne <: Refines BmapAllocAll BmapAllocOne.
 
 Obligation Tactic := Tactics.program_simpl; omega'.
 
-(* XXX *)
+Definition bmalloc_helper (R:Type) (bn:blockmapnum) (oa:option blockmapoff)
+                          (rxok:(blockmapnum*blockmapoff)->BmapAllocOne.Prog R)
+                          (rxfail:BmapAllocOne.Prog R) : BmapAllocOne.Prog R :=
+  match oa with
+  | None => rxfail
+  | Some off => rxok (bn, off)
+  end.
 
+Program Fixpoint bmalloc (R:Type) (n:nat) (NOK:n<=NBlockMap)
+                         (rx:option (blockmapnum*blockmapoff)->BmapAllocOne.Prog R) :=
+  match n with
+  | O => rx None
+  | S x =>
+    oa <- BmapAllocOne.Alloc x;
+    bmalloc_helper R x oa
+                   (fun x => rx (Some x))
+                   (bmalloc R x _ rx)
+  end.
+
+Program Fixpoint Compile {R:Type} (p:BmapAllocAll.Prog R) : BmapAllocOne.Prog R :=
+  match p with
+  | BmapAllocAll.Alloc rx =>
+    bmalloc R NBlockMap _ (fun x => Compile (rx x))
+  | BmapAllocAll.Free bn off rx =>
+    BmapAllocOne.Free bn off ;; (Compile (rx tt))
+  | BmapAllocAll.Return r =>
+    BmapAllocOne.Return r
+  end.
+
+Inductive statematch : BmapAllocAll.State -> BmapAllocOne.State -> Prop :=
+  | Match: forall s,
+    statematch s s.
+Definition StateMatch := statematch.
+Hint Constructors statematch.
+
+Lemma bmalloc_fail:
+  forall R n Hn rx d,
+  (~exists bn off, BmapAllocOne.freebit (d bn) off) ->
+  star (BmapAllocOne.Step R)
+    (PS (bmalloc R n Hn rx) d)
+    (PS (rx None) d).
+Proof.
+  induction n; intros.
+  - apply star_refl.
+  - eapply star_step; [apply BmapAllocOne.StepAllocOut|].
+    + unfold not; intros. apply H; clear H. eexists (exist _ n _). apply H0.
+    + cbv beta.
+      fold bmalloc. unfold bmalloc_helper. apply IHn. auto.
+Qed.
+
+Lemma bmalloc_ok:
+  forall R n Hn rx d bn off,
+  highest_below (fun bn' => exists off', BmapAllocOne.freebit (d bn') off') n bn ->
+  highest (BmapAllocOne.freebit (d bn)) off ->
+  star (BmapAllocOne.Step R)
+    (PS (bmalloc R n Hn rx) d)
+    (PS (rx (Some (bn, off)))
+        (setidx eq_blockmapnum_dec d bn
+         (setidx eq_blockmapoff_dec (d bn) off InUse))).
+Proof.
+  induction n; intros.
+  - destruct H. crush.
+  - case_eq (eq_nat_dec (proj1_sig bn) n); intros.
+    + eapply star_step; [apply BmapAllocOne.StepAllocOK|];
+      subst; repeat rewrite exist_proj_sig.
+      * eauto.
+      * apply star_refl.
+    + eapply star_step; [apply BmapAllocOne.StepAllocOut|];
+      [ | apply IHn; auto; apply highest_below_next with (Hbound:=Hn); auto ];
+      ( unfold not; intros;
+        destruct H; Tactics.destruct_pairs; apply H3;
+        eexists (exist _ n _);
+        split; [omega'|eauto] ).
+Qed.
+
+Theorem FSim:
+  forall R,
+  forward_simulation (BmapAllocAll.Step R) (BmapAllocOne.Step R).
+Proof.
+  intros; exists (progmatch Compile statematch); intros.
+
+  repeat match goal with
+  | [ x: progmatch _ _ _ _ |- _ ] => inversion x; clear x; subst
+  | [ x: statematch _ _ |- _ ] => inversion x; clear x; subst
+  end.
+
+  match goal with
+  | [ x: BmapAllocAll.Step _ _ _ |- _ ] => inversion x; clear x; subst
+  end.
+
+  - (* Alloc Some *)
+    econstructor; split.
+    + apply bmalloc_ok; [ apply highest_below_bound | ]; eauto.
+    + crush.
+
+  - (* Alloc None *)
+    econstructor; split.
+    + apply bmalloc_fail; auto.
+    + crush.
+
+  - (* Free *)
+    econstructor; split.
+    + eapply star_step; [constructor|].
+      apply star_refl.
+    + crush.
+Qed.
 
 End BmapAllocAllToAllocOne.
